

## Derivatives

### Ex 1.

Calculate the derivatives of the functions

1)  $y = \frac{1}{3}x^3 - \frac{3}{2}x^4 + \frac{13}{5}x^5 - 2x^6$

2)  $y = 5x^{15} - x^2 + \frac{1}{3}x - 2$

3)  $y = ax^3 + \frac{b}{x} + c$

4)  $y = \frac{4}{x^3}$

5)  $y = 9x^7 + 3x^{-5} - 3x^{-11}$

6)  $y = 3x^{7/3} - 4x^{13/4} + \frac{4}{7}x^{-1/2} + 7^{3/2}$

7)  $y = \sqrt[3]{x^2}$

8)  $y = 5\sqrt[3]{x^7}$

9)  $y = 3\sqrt[3]{x} - x^3 + \frac{2}{3}\sqrt[3]{x^4}$

10)  $y = \sqrt{x} - 5\sqrt[3]{x^2} - 2\sqrt{x^3}$

11)  $y = \frac{2}{\sqrt{x}} - \frac{3}{\sqrt{x^3}}$

12)  $y = \frac{5}{7\sqrt[3]{x}} - 2x^7 + \frac{3}{2\sqrt{x}}$

13)  $x = t^3\sqrt{t}$

14)  $y = \frac{2}{x^3\sqrt{x}}$

15)  $y = (2\sqrt[3]{x^2} - x)(4\sqrt[3]{x^4} + 2\sqrt[3]{x^5} + x^2)$

16)  $y = (4x^2 - 2x\sqrt{x} + x)(2x + \sqrt{x})$

17)  $y = \frac{3}{3x-2}$

18)  $y = \frac{5}{2x^2-5x+1}$

19)  $y = \frac{3x^2}{7x^5-x+2}$

20)  $y = \frac{8x^3}{x^3+x-1}$

21)  $y = \frac{x+1}{x-1}$

22)  $y = \frac{5x^2+x-2}{x^2+7}$

23)  $y = \frac{x^2-2x+3}{x^2+2x-3}$

24)  $y = \frac{3}{(1-x^2)(1-2x^3)}$

25)  $y = \frac{\sqrt[3]{x}}{1-\sqrt[3]{x}}$

26)  $z = \frac{1+\sqrt{t}}{1+\sqrt{2t}}$

27)  $s = (3t+1)^7$

28)  $v = (4z^2 - 5z + 13)^5$

29)  $x = (\frac{1}{t} + 4)^4$

30)  $s = (\frac{7t^2 - \frac{t}{2} + 6}{t})^6$

31)  $y = \sqrt{x^2 - 4}$

32)  $z = \sqrt{ax^2 + bx + c}$

- 33)  $y = \frac{1}{\sqrt{2-3t}}$
- 34)  $s = \frac{1}{\sqrt{6t-t^2}}$
- 35)  $y = \frac{1}{\sqrt[3]{(2-x^3)^4}}$
- 36)  $y = \frac{a}{\sqrt[r]{(a+bx)^r}}$
- 37)  $y = \frac{1}{(b-x^n)^m}$
- 38)  $y = \sqrt[4]{(x-1)^3}$
- 39)  $u = \frac{1}{v-\sqrt{a^2+b^2}}$
- 40)  $y = \sqrt{\frac{a-x}{a^2-x^2}}, a > 0$
- 41)  $v = \frac{z}{\sqrt{a^2-z^2}}$
- 42)  $y = \frac{3\sqrt{x}}{x^2+1}$
- 43)  $y = \frac{x^2}{\sqrt[3]{x^3+1}}$
- 44)  $z = \sqrt{\frac{x^2-3x+2}{x^2-7x+12}}$
- 45)  $z = \sqrt{\frac{a^2-x^2}{a^2+x^2}}$
- 46)  $s = \sqrt{\frac{1-\sqrt{t}}{1+\sqrt{t}}}$
- 47)  $u = \frac{\sqrt{1+v}-\sqrt{1-v}}{\sqrt{1+v}+\sqrt{1-v}}$
- 48)  $y = u(x)v(x)w(x)$
- 49)  $v = \cos \frac{t}{a}, a \neq 0$
- 50)  $x = a \sin bt$
- 51)  $y = a \sin \frac{a}{x}$
- 52)  $z = 2x + \sin 2x$
- 53)  $s = \sin^2 3t$
- 54)  $v = 4 \cos^5 \frac{t}{4}$
- 55)  $s = \frac{1}{\cos^4 t}$
- 56)  $v = \frac{5}{\sin^3 2t}$
- 57)  $s = \frac{\sin t + \cos t}{2 \sin 2t}$
- 58)  $z = \frac{\sin \alpha}{\alpha} + \frac{\alpha}{\sin \alpha}$
- 59)  $y = \frac{x \sin x}{1+\operatorname{tg} x}$
- 60)  $y = \frac{x}{\sin x + \cos x}$
- 61)  $y = \cos x - \frac{1}{3} \cos^3 x$
- 62)  $y = \frac{1}{3} \sin^3 x - \frac{2}{5} \sin^5 x + \frac{1}{7} \sin^7 x$
- 63)  $y = \operatorname{tg}^4 \sqrt{x}$
- 64)  $y = 3 \operatorname{ctg} x + \operatorname{ctg}^3 x$
- 65)  $y = e^{ax}(a \sin x - \cos x)$
- 66)  $y = x^2 e^{2x} \sin x$

- 67)  $y = \cos^2 \frac{1}{\sqrt{x}}$
- 68)  $y = 2 \sin^4 \frac{3}{\sqrt{x}}$
- 69)  $y = \frac{\sin^2 x}{\cos^7 x} - \frac{2}{5 \cos^5 x}$
- 70)  $y = \frac{3 \cos^2 x}{\sin^4 x}$
- 71)  $y = \sqrt{\sin x + \sqrt{x + 2\sqrt{x}}}$
- 72)  $y = \sqrt{1 + \operatorname{tg}(x + \frac{1}{x})}$
- 73)  $z = \frac{3 \operatorname{tg} u - \operatorname{tg}^3 u}{1 - 3 \operatorname{tg}^2 u}$
- 74)  $z = \operatorname{tg} u - \operatorname{ctg} u - 2u$
- 75)  $y = (4 \sin x - 8 \sin^3 x) \cos x$
- 76)  $y = \operatorname{arctg} 3x$
- 77)  $y = 7 \operatorname{arctg} \frac{x}{2}$
- 78)  $x = \arcsin(1 - t)$
- 79)  $x = \arccos \sqrt{1 - t^2}$
- 80)  $x = \arcsin \sqrt{t^3}$
- 81)  $x = \arcsin \frac{1}{t}$
- 82)  $y = x \arcsin x + \sqrt{1 - x^2}, 0 < x < 1$
- 83)  $x = \arcsin(2t\sqrt{1 - t^2})$
- 84)  $y = \operatorname{arctg}(x - \sqrt{x^2 + 1})$
- 85)  $y = \operatorname{arctg} \sqrt{x^2 - 1} - \frac{\ln x}{\sqrt{x^2 - 1}}$
- 86)  $y = x \operatorname{arctg} x - \frac{1}{2} \ln(x^2 + 1)$
- 87)  $y = \frac{1}{6} x^5 \operatorname{arctg} x - \frac{1}{24} x^4 + \frac{1}{12} x^2 - \frac{1}{12} \ln(1 + x^2)$
- 88)  $y = \arcsin \frac{x}{\sqrt{1+x^2}}$
- 89)  $y = \arccos \sqrt{\frac{1-x^2}{1+x^2}}$
- 90)  $y = \operatorname{arctg} \sqrt{\frac{1-x}{1+x}}$
- 91)  $y = \operatorname{arctg} \frac{1+x}{1-x}, x \neq 1$
- 92)  $y = \operatorname{arctg} \frac{x}{1+\sqrt{1+x^2}}$
- 93)  $y = \operatorname{arctg} \frac{\sqrt{1+x^2}-1}{x}$
- 94)  $y = x^3 \operatorname{arctg}^3 x$
- 95)  $z = \frac{\arcsin 4y}{1-4y}$
- 96)  $y = \frac{4}{\sqrt{3}} \operatorname{arctg} \left[ \frac{1}{\sqrt{3}} (2 \operatorname{tg} \frac{x}{2} + 1) \right] - x$
- 97)  $y = \frac{1}{\sqrt{a^2 - b^2}} \arcsin \frac{a \cos x + b}{a + b \cos x}$
- 98)  $y = e^{3x}$
- 99)  $y = 5e^{4x}$
- 100)  $y = e^{x^2} f(x)$

- 101)  $y = 3e^{-2x}g(x)$
- 102)  $y = e^{\sin x}$
- 103)  $y = 5e^{\cos x}$
- 104)  $y = e^{\cos^2 x}$
- 105)  $y = 3e^{2\sin^3 x}$
- 106)  $z = (v^3 - 3v^2 + 6v - 6)e^v$
- 107)  $z = (10x^2 - 1)e^{3x}$
- 108)  $z = \frac{(2x-1)e^x}{2\sqrt{x}}$
- 109)  $y = (x + k\sqrt{1-x^2})e^{k \arcsin x}$
- 110)  $y = 5^x + 2^x$
- 111)  $y = 3^x x^3$
- 112)  $y = 2^x \cdot 7^x - 1$
- 113)  $y = 5 \cdot 10^{3x}$
- 114)  $y = a^{2x} x^n, a > 0$
- 115)  $y = \ln 3x$
- 116)  $y = 7 \cdot 5^{10x}$
- 117)  $z = \ln \frac{30}{x+3}$
- 118)  $y = 5 \ln 10x$
- 119)  $s = \ln(t + \sqrt{t^2 + 1})$
- 120)  $z = 3 \ln \frac{5}{x-2}$
- 121)  $s = \ln \sqrt{\frac{1+t}{1-t}}$
- 122)  $y = 2 \ln \frac{3}{t+\sqrt{t^2-4}}$
- 123)  $y = \ln |\ln |x||$
- 124)  $y = \ln \frac{a+b \operatorname{tg} x}{a-b \operatorname{tg} x}$
- 125)  $y = \ln \operatorname{tg}(\frac{\pi}{4} + \frac{x}{2}), 0 < x < \frac{\pi}{2}$
- 126)  $y = (\ln \cos \frac{x}{2})^2$
- 127)  $y = \ln \sqrt{\frac{1+\sin x}{1-\sin x}}$
- 128)  $y = 15 \ln \operatorname{tg} \frac{x}{2} + \frac{\cos x}{\sin^4 x} (8 \cos^4 x - 25 \cos^2 x + 15)$
- 129)  $y = \ln \sin x$
- 130)  $y = \ln \frac{1+\sqrt{x}}{1-\sqrt{x}}, 0 \leq x < 1$
- 131)  $y = \ln(1 + \frac{a}{x})$
- 132)  $y = \ln(e^{mx} + e^{-mx})$
- 133)  $y = \log_x \ln x.$
- 134)  $y = \log_x a.$
- 135)  $y = x^{5x}, x > 0$
- 136)  $y = 10x^{-3x}, x > 0$

- 137)  $y = x^{\sin x}, x > 0$
- 138)  $y = 3x^{\cos x}, x > 0$
- 139)  $y = (\frac{a}{x})^x, a > 0, x > 0$
- 140)  $y = x^{1/x}, x > 0$
- 141)  $y = a^{\ln x}, a > 0, x > 0$
- 142)  $y = 5^{\sin 2x}, x > 0$
- 143)  $y = x^{\ln x}, x > 0$ ; explain the result.
- 144)  $y = (\sin x)^{\cos x}, 0 < x < \frac{\pi}{2}$
- 145)  $y = (\operatorname{arctg} x)^x, x > 0$
- 146)  $y = (\operatorname{tg} x)^{\sin x}, 0 < x < \frac{\pi}{2}$
- 147)  $y = (\operatorname{tg} x)^{1/\cos x}, 0 < x < \frac{\pi}{2}$
- 148)  $y = (\cos x)^{\operatorname{ctg} x}, 0 < x < \frac{\pi}{2}$
- 149)  $y = e^{e^x}$
- 150)  $y = x^{e^x}, x > 0$
- 151)  $y = x^{x^x}, x > 0$
- 152)  $y = (1 + \frac{1}{x})^x$
- 153)  $y = x^{\sqrt{\frac{1}{x}}}$